VersionControl.lean
@@ -1,3 +1,9 @@
 -- This module serves as the root of the `VersionControl` library.
 -- Import modules here that should be built as part of the library.
 import VersionControl.Basic
+import VersionControl.Defns
+import VersionControl.JsonParse
+import VersionControl.Semantics
+import VersionControl.Conflict
+import VersionControl.History
+import VersionControl.FullMerge
